fragments.v
@@ -1,18 +1,59 @@
-Set Warnings "-notation-overridden,-parsing,-deprecated-hint-without-locality".
 From Coq Require Import Arith.Arith.
 From Coq Require Import Arith.EqNat.
 From Coq Require Import Init.Nat.
 From Coq Require Import Lia.
 From Coq Require Import Lists.List. Import ListNotations.
 
-Theorem update_same : forall (A : Type) (m : partial_map A) x v,
-  m x = Some v ->
-  (x |-> v ; m) = m.
+Definition relation (X : Type) := X -> X -> Prop.
+
+Definition deterministic {X : Type} (R : relation X) :=
+  forall x y1 y2 : X, R x y1 -> R x y2 -> y1 = y2.
+
+Definition normal_form {X : Type}
+              (R : relation X) (t : X) : Prop :=
+  ~ exists t', R t t'.
+
+
+Inductive multi {X : Type} (R : relation X) : relation X :=
+  | multi_refl : forall (x : X), multi R x x
+  | multi_step : forall (x y z : X),
+                    R x y ->
+                    multi R y z ->
+                    multi R x z.
+
+
+Theorem multi_R : forall (X : Type) (R : relation X) (x y : X),
+    R x y -> (multi R) x y.
 Proof.
-  intros A m x v H. unfold update. rewrite <- H.
-  apply t_update_same.
+  intros X R x y H.
+  apply multi_step with y.
+  - apply H.
+  - apply multi_refl.
 Qed.
 
+Theorem multi_trans :
+  forall (X : Type) (R : relation X) (x y z : X),
+      multi R x y  ->
+      multi R y z ->
+      multi R x z.
+Proof.
+  intros X R x y z G H.
+  induction G.
+    - (* multi_refl *) assumption.
+    - (* multi_step *)
+      apply multi_step with y.
+      + assumption.
+      + apply IHG. assumption.
+Qed.
+
+
+Tactic Notation "print_goal" :=
+  match goal with |- ?x => idtac x end.
+
+Tactic Notation "normalize" :=
+  repeat (print_goal; eapply multi_step ;
+            [ (eauto 10; fail) | simpl]);
+  apply multi_refl.
 
 Definition deterministic {X : Type} (R : relation X) :=
   forall x y1 y2 : X, R x y1 -> R x y2 -> y1 = y2.
@@ -25,23 +66,17 @@ Ltac solve_by_inverts n :=
       match n with S (S (?n')) => subst; solve_by_inverts (S n') end ]
   end end.
 
-
-
 Ltac solve_by_invert :=
   solve_by_inverts 1.
-
-
 
 Definition normal_form {X : Type}
               (R : relation X) (t : X) : Prop :=
   ~ exists t', R t t'.
 
-
 Lemma value_is_nf : forall v,
   value v -> normal_form step v.
 Lemma nf_is_value : forall t,
   normal_form step t -> value t.
-
 
 Inductive multi {X : Type} (R : relation X) : relation X :=
   | multi_refl : forall (x : X), multi R x x
@@ -58,8 +93,6 @@ Proof.
   - apply multi_refl.
 Qed.
 
-
-
 Theorem multi_trans :
   forall (X : Type) (R : relation X) (x y z : X),
       multi R x y  ->
@@ -75,10 +108,6 @@ Proof.
       + apply IHG. assumption.
 Qed.
 
-
-
-
-
 Definition step_normal_form := normal_form step.
 
 Definition normal_form_of (t t' : tm) :=
@@ -90,15 +119,10 @@ Definition normalizing {X : Type} (R : relation X) :=
   forall t, exists t',
     (multi R) t t' /\ normal_form R t'.
 
-
-Tactic Notation "print_goal" := idtac.
-
-
 Tactic Notation "normalize" :=
   repeat (print_goal; eapply multi_step ;
             [ (eauto 10; fail) | simpl]);
   apply multi_refl.
-
 
 Notation step_normal_form := (normal_form step).
 
@@ -110,7 +134,6 @@ Hint Unfold stuck : core.
 Definition nf : tm -> Prop := normal_form step.
 
 Theorem nf_if_value (t : tm) : value t -> nf t.
-
 
 Ltac find_value_step :=
   match goal with
@@ -125,24 +148,11 @@ Ltac find_value_step_aggr :=
 
 Theorem type_unique t : forall Gamma T1 T2, Gamma |-- t \in T1 -> Gamma |-- t \in T2 -> T1 = T2.
 
-
 Definition normalizing (t : tm) := exists t', t -->* t' /\ nf t'.
 
 Definition context_value := list (string * tm * ty).
 
-Ltac search_eq :=
-  subst;
-  try match goal with
-  H : (?s |-> _ ; _) ?s = Some _ |- _
-  => rewrite update_eq in H; injection H as H; subst
-  end;
-  try match goal with
-  H : (?s |-> _ ; _) ?t = _, H2 : ?s <> ?t |- _
-  => rewrite update_neq in H; eauto
-  end.
-
 Lemma good_filt : forall s Gamma, good Gamma -> good (filt s Gamma).
-
 
 Ltac get_norm :=
   repeat match goal with
