Lemma.v
@@ -1,0 +1,44 @@
+From Lambda Require Import Map.
+From Lambda Require Import Syntax.
+From Lambda Require Import LibTactics.
+From Coq Require Import Classes.CEquivalence.
+From Coq Require Classes.CMorphisms.
+Set Default Goal Selector "!".
+
+Lemma weaken t T :
+  forall (G1 : context), G1 |-- t \in T ->
+  forall (G2 : context), includedin G1 G2 ->
+  G2 |-- t \in T.
+Proof.
+  introv HT; induction HT; intros; eauto 7 using includedin_update.
+Defined.
+
+Corollary weaken_empty t T :
+  empty |-- t \in T -> forall G, G |-- t \in T.
+Proof.
+  intros. eapply weaken; eauto. discriminate.
+Defined.
+
+Corollary has_type_extensionality :
+  forall G1 G2 t T,
+  G1 ~ G2 -> G1 |-- t \in T -> G2 |-- t \in T.
+Proof.
+  introv Hext HT. eapply weaken; eauto. congruence.
+Defined.
+
+Global Instance equiv_rel {A} :
+  Equivalence (@mapeq A) :=
+{|
+  Equivalence_Reflexive := mapeq_refl;
+  Equivalence_Symmetric := mapeq_sym;
+  Equivalence_Transitive := mapeq_trans
+|}.
+
+Global Instance update_morphism {A} x v :
+  CMorphisms.Proper (CMorphisms.respectful (@mapeq A) (@mapeq A)) (update x v) := fun _ _ => mapeq_cong _ _ _ _.
+
+Global Instance has_type_morphism t T :
+  CMorphisms.Proper (CMorphisms.respectful mapeq iffT) (has_type t T) :=
+  (fun m1 m2 Hequ =>
+   (has_type_extensionality m1 m2 t T Hequ,
+   has_type_extensionality m2 m1 t T (mapeq_sym m1 m2 Hequ))).
